IMPState namespacing and Monad simp attributes

LeanIMP/IMPState.lean
@@ -1,241 +1,227 @@
 import LeanIMP.Basic
 
 
+namespace IMPState
 
-def IMPState.ext_eq {α: Type} [BEq α] (s1 s2 : IMPState α) : Prop :=
-  forall (k : α), s1.lookup k = s2.lookup k
+  def ext_eq {α: Type} [BEq α] (s1 s2 : IMPState α) : Prop :=
+    forall (k : α), s1.lookup k = s2.lookup k
 
-theorem IMPState.lookup_congr {α: Type} [BEq α] (k : α) {s1 s2 : IMPState α} (h : IMPState.ext_eq s1 s2) :
-  s1.lookup k = s2.lookup k :=
-  h k
+  theorem lookup_congr {α: Type} [BEq α] (k : α) {s1 s2 : IMPState α} (h : ext_eq s1 s2) :
+    s1.lookup k = s2.lookup k :=
+    h k
 
-theorem IMPState.ext_eq_reflexive {α: Type} [BEq α] (s : IMPState α) : IMPState.ext_eq s s :=
-  by
-    unfold IMPState.ext_eq
-    intros k
-    eq_refl
-
-theorem IMPState.ext_eq_symmetric {α: Type} [BEq α] {s1 s2 : IMPState α} : (IMPState.ext_eq s1 s2) -> (IMPState.ext_eq s2 s1)  :=
-  by
-    unfold IMPState.ext_eq
-    intros ass k
-    symm
-    apply ass
-
-
-theorem IMPState.ext_eq_transitive {α: Type} [BEq α] {s1 s2 s3 : IMPState α} : (IMPState.ext_eq s1 s2) -> (IMPState.ext_eq s2 s3) -> (IMPState.ext_eq s1 s3)  :=
-  by
-    intros ass1 ass2
-    unfold IMPState.ext_eq
-    intros k
-    rw [ass1]
-    apply ass2
-
-
-instance IMPStateEquivalence {α: Type} [beq : BEq α] : Equivalence (@IMPState.ext_eq α beq) where
-  refl := IMPState.ext_eq_reflexive
-  symm := IMPState.ext_eq_symmetric
-  trans := IMPState.ext_eq_transitive
-
-
-instance IMPStateSetoid (α: Type) [BEq α] : Setoid (IMPState α) where
-  r := IMPState.ext_eq
-  iseqv := IMPStateEquivalence
-
-def IMPStateQ (α: Type) [BEq α] := Quotient (IMPStateSetoid α)
-
-
-theorem IMPState.update_twice_eq_update_once {α: Type} [BEq α] (s : IMPState α) (k_update : α) (v1 v2 : Nat) :
-  Quotient.mk' (IMPState.update (s.update k_update v1) k_update v2) = Quotient.mk' (s.update k_update v2) :=
+  theorem ext_eq_reflexive {α: Type} [BEq α] (s : IMPState α) : ext_eq s s :=
     by
-      have is_ext_eq : ext_eq (IMPState.update (s.update k_update v1) k_update v2) (s.update k_update v2) := by
-        intros k
-        cases h_lem_bool: k == k_update with
-          | true =>
-            unfold List.lookup
-            unfold update
-            simp
-            rw [h_lem_bool]
-          | false =>
-            unfold List.lookup
-            unfold update
-            simp
-            rw [h_lem_bool]
-            simp
-            unfold List.lookup
-            rw [h_lem_bool]
-            simp
-            match s with
-              | List.nil => simp
-              | List.cons head tail =>
-                simp
-                rw [List.lookup]
+      unfold ext_eq
+      intros k
+      eq_refl
 
-      exact Quotient.sound is_ext_eq
+  theorem ext_eq_symmetric {α: Type} [BEq α] {s1 s2 : IMPState α} : (ext_eq s1 s2) -> (ext_eq s2 s1)  :=
+    by
+      unfold ext_eq
+      intros ass k
+      symm
+      apply ass
 
 
-theorem IMPState.update_unrelated_eq_update_once {α: Type} [BEq α] (s : IMPState α) (k1 k2: α) (v2 : Nat) (k1_neq_k2 : ¬(k1 == k2)) :
-  (IMPState.update s k2 v2).lookup k1 = s.lookup k1 :=
-  by
-    unfold update
-    unfold List.lookup
-    cases h_eq_bool : (k1 == k2) with
-      | true =>
-        have eq : k1 == k2 := by
-          exact h_eq_bool
-        contradiction
-      | false =>
-        match s with
-          | List.nil => simp
-          | List.cons head tail =>
-            simp
-            conv =>
-              lhs
+  theorem ext_eq_transitive {α: Type} [BEq α] {s1 s2 s3 : IMPState α} : (ext_eq s1 s2) -> (ext_eq s2 s3) -> (ext_eq s1 s3)  :=
+    by
+      intros ass1 ass2
+      unfold ext_eq
+      intros k
+      rw [ass1]
+      apply ass2
+
+
+  instance IMPStateEquivalence {α: Type} [beq : BEq α] : Equivalence (@ext_eq α beq) where
+    refl := ext_eq_reflexive
+    symm := ext_eq_symmetric
+    trans := ext_eq_transitive
+
+
+  instance IMPStateSetoid (α: Type) [BEq α] : Setoid (IMPState α) where
+    r := ext_eq
+    iseqv := IMPStateEquivalence
+
+  def IMPStateQ (α: Type) [BEq α] := Quotient (IMPStateSetoid α)
+
+  theorem update_twice_eq_update_once {α: Type} [BEq α] (s : IMPState α) (k_update : α) (v1 v2 : Nat) :
+    Quotient.mk' (update (s.update k_update v1) k_update v2) = Quotient.mk' (s.update k_update v2) :=
+      by
+        have is_ext_eq : ext_eq (update (s.update k_update v1) k_update v2) (s.update k_update v2) := by
+          intros k
+          cases h_lem_bool: k == k_update with
+            | true =>
               unfold List.lookup
+              unfold update
+              simp
+              rw [h_lem_bool]
+            | false =>
+              unfold List.lookup
+              unfold update
+              simp
+              rw [h_lem_bool]
+              simp
+              unfold List.lookup
+              rw [h_lem_bool]
+              simp
+              match s with
+                | List.nil => simp
+                | List.cons head tail =>
+                  simp
+                  rw [List.lookup]
+
+        exact Quotient.sound is_ext_eq
 
 
-
-theorem IMPState.prepend_update_eq_reverse_append {α: Type} [BEq α] (s1 s2: IMPState α) :
-  s1.prepend_updates s2 = s2.append s1 :=
-  by
-    induction s2 generalizing s1 with
-    | nil =>
-      unfold prepend_updates
-      simp
-    | cons head tail ih =>
-      -- step case
-      unfold prepend_updates
-      simp
-      unfold IMPState.update
-      unfold List.foldr
-      simp
-      match tail with
-        | List.nil => simp
-        | List.cons _ _ =>
-          simp
-
-theorem IMPState.prepend_update_eq_reverse_Happend {α: Type} [BEq α] (s1 s2: IMPState α) :
-  s1.prepend_updates s2 = s2 ++ s1 :=
-  by
-    exact IMPState.prepend_update_eq_reverse_append s1 s2
-
-
-theorem IMPState.update_unrelated_eq_update_list {α: Type} [BEq α] [PartialEquivBEq α] (s1 s2 : IMPState α) (k: α) (s2_does_not_contain : IMPState.does_not_contain s2 k) :
-  (s1.prepend_updates s2).lookup k = s1.lookup k :=
-  by
-    induction s2 generalizing s1 with
-    | nil =>
-      unfold prepend_updates
-      simp
-    | cons head tail ih =>
-      unfold prepend_updates
-      simp
+  theorem update_unrelated_eq_update_once {α: Type} [BEq α] (s : IMPState α) (k1 k2: α) (v2 : Nat) (k1_neq_k2 : ¬(k1 == k2)) :
+    (update s k2 v2).lookup k1 = s.lookup k1 :=
+    by
       unfold update
-      have head_is_not : ¬(head.fst == k) := by
-        apply s2_does_not_contain.left
-      have head_is_not_symm : (k == head.fst) = false := by
+      unfold List.lookup
+      cases h_eq_bool : (k1 == k2) with
+        | true =>
+          have eq : k1 == k2 := by
+            exact h_eq_bool
+          contradiction
+        | false =>
+          match s with
+            | List.nil => simp
+            | List.cons head tail =>
+              simp
+              conv =>
+                lhs
+                unfold List.lookup
+
+
+
+  theorem prepend_update_eq_reverse_append {α: Type} [BEq α] (s1 s2: IMPState α) :
+    s1.prepend_updates s2 = s2.append s1 :=
+    by
+      induction s2 generalizing s1 with
+      | nil =>
+        unfold prepend_updates
+        simp
+      | cons head tail ih =>
+        -- step case
+        unfold prepend_updates
+        simp
+        unfold update
+        unfold List.foldr
+        simp
+        match tail with
+          | List.nil => simp
+          | List.cons _ _ =>
+            simp
+
+  theorem prepend_update_eq_reverse_Happend {α: Type} [BEq α] (s1 s2: IMPState α) :
+    s1.prepend_updates s2 = s2 ++ s1 :=
+    by
+      exact prepend_update_eq_reverse_append s1 s2
+
+
+  theorem update_unrelated_eq_update_list {α: Type} [BEq α] [PartialEquivBEq α] (s1 s2 : IMPState α) (k: α) (s2_does_not_contain : does_not_contain s2 k) :
+    (s1.prepend_updates s2).lookup k = s1.lookup k :=
+    by
+      induction s2 generalizing s1 with
+      | nil =>
+        unfold prepend_updates
+        simp
+      | cons head tail ih =>
+        unfold prepend_updates
+        simp
+        unfold update
+        have head_is_not : ¬(head.fst == k) := by
+          apply s2_does_not_contain.left
+        have head_is_not_symm : (k == head.fst) = false := by
+          conv =>
+            arg 1
+            rw [BEq.comm]
+          exact Eq.symm ((fun {a b} ↦ Bool.not_not_eq.mp) fun a ↦ head_is_not (id (Eq.symm a)))
+        conv =>
+          lhs
+          unfold List.lookup
+        rw [head_is_not_symm]
+        simp
+        rw [<- prepend_update_eq_reverse_Happend]
+        apply ih
+        exact s2_does_not_contain.right
+
+  theorem eval_int_is_pure {α: Type} [BEq α] (s: IMPState α) (expr : NatExpr α) :
+    (evalNatExpr expr) s = (((evalNatExpr expr) s).fst, s) :=
+    by
+      induction expr generalizing s with
+      | var key =>
+        simp [evalNatExpr]
+        match List.lookup key s with
+          | none => eq_refl
+          | some _ => eq_refl
+      | const c =>
+        simp [evalNatExpr]
+      | add a b ih_a ih_b
+      | sub a b ih_a ih_b
+      | mul a b ih_a ih_b =>
+        simp [evalNatExpr]
+        rw [ih_a s]
         conv =>
           arg 1
-          rw [BEq.comm]
-        exact Eq.symm ((fun {a b} ↦ Bool.not_not_eq.mp) fun a ↦ head_is_not (id (Eq.symm a)))
-      conv =>
-        lhs
-        unfold List.lookup
-      rw [head_is_not_symm]
-      simp
-      rw [<- IMPState.prepend_update_eq_reverse_Happend]
-      apply ih
-      exact s2_does_not_contain.right
+          dsimp
+        simp
+        rw [ih_b s]
 
 
-macro "simp_monad" : tactic =>
-  `(tactic| simp [Bind.bind, Monad.toBind, StateT.pure, StateT.run, StateT.instMonad, StateT.bind, StateT.map, MonadState.get, getThe, MonadStateOf.get, StateT.get, set, StateT.set, Id.run])
+  theorem eval_bool_is_pure {α: Type} [BEq α] (s: IMPState α) (expr : BoolExpr α) :
+    (evalBoolExpr expr) s = (((evalBoolExpr expr) s).fst, s) :=
+    by
+      induction expr generalizing s with
+      | var key =>
+        simp [evalBoolExpr]
+        match List.lookup key s with
+          | none => eq_refl
+          | some val =>
+            match h: val with
+              | 0 =>
+                rfl
+              | Nat.succ n =>
+                rfl
+      | const c =>
+        simp [evalBoolExpr]
+      | eq a b
+      | neq a b
+      | lt a b
+      | leq a b
+      | gt a b
+      | geq  =>
+        simp [evalBoolExpr]
+        rw [eval_int_is_pure]
+        simp
+        rw [eval_int_is_pure]
+      | and a b ih_a ih_b =>
+        simp [evalBoolExpr]
+        rw [ih_a s]
+        conv =>
+          arg 1
+          dsimp
+        match (evalBoolExpr a s) with
+          | (true, _) =>
+            simp
+            exact (ih_b s)
+          | (false, _) =>
+            simp
+      | or a b ih_a ih_b =>
+        simp [evalBoolExpr]
+        rw [ih_a s]
+        conv =>
+          arg 1
+          dsimp
+        match (evalBoolExpr a s) with
+          | (true, _) =>
+            simp
+          | (false, _) =>
+            simp
+            exact (ih_b s)
+      | not a ih_a =>
+        simp [evalBoolExpr]
+        rw [ih_a s]
 
-theorem IMPState.eval_int_is_pure {α: Type} [BEq α] (s: IMPState α) (expr : NatExpr α) :
-  (evalNatExpr expr) s = (((evalNatExpr expr) s).fst, s) :=
-  by
-    induction expr generalizing s with
-    | var key =>
-      simp [evalNatExpr]
-      simp_monad
-      match List.lookup key s with
-        | none => eq_refl
-        | some _ => eq_refl
-    | const c =>
-      simp [evalNatExpr]
-      simp_monad
-    | add a b ih_a ih_b
-    | sub a b ih_a ih_b
-    | mul a b ih_a ih_b =>
-      simp [evalNatExpr]
-      simp_monad
-      rw [ih_a s]
-      conv =>
-        arg 1
-        dsimp
-      simp_monad
-      rw [ih_b s]
-
-
-theorem IMPState.eval_bool_is_pure {α: Type} [BEq α] (s: IMPState α) (expr : BoolExpr α) :
-  (evalBoolExpr expr) s = (((evalBoolExpr expr) s).fst, s) :=
-  by
-    induction expr generalizing s with
-    | var key =>
-      simp [evalBoolExpr]
-      simp_monad
-      match List.lookup key s with
-        | none => eq_refl
-        | some val =>
-          match h: val with
-            | 0 =>
-              rfl
-            | Nat.succ n =>
-              rfl
-    | const c =>
-      simp  [evalBoolExpr]
-      simp_monad
-    | eq a b
-    | neq a b
-    | lt a b
-    | leq a b
-    | gt a b
-    | geq  =>
-      simp [evalBoolExpr]
-      simp_monad
-      rw [eval_int_is_pure]
-      simp
-      rw [eval_int_is_pure]
-    | and a b ih_a ih_b =>
-      simp [evalBoolExpr]
-      simp_monad
-      rw [ih_a s]
-      conv =>
-        arg 1
-        dsimp
-      simp_monad
-      match (evalBoolExpr a s) with
-        | (true, _) =>
-          simp
-          exact (ih_b s)
-        | (false, _) =>
-          simp_monad
-    | or a b ih_a ih_b =>
-      simp [evalBoolExpr]
-      simp_monad
-      rw [ih_a s]
-      conv =>
-        arg 1
-        dsimp
-      simp_monad
-      match (evalBoolExpr a s) with
-        | (true, _) =>
-          simp
-          simp_monad
-        | (false, _) =>
-          simp
-          exact (ih_b s)
-    | not a ih_a =>
-      simp [evalBoolExpr]
-      simp_monad
-      rw [ih_a s]
+end IMPState
